-

coq/Puiseux_base.v
@@ -1,4 +1,4 @@
-(* $Id: Puiseux_base.v,v 1.27 2013-06-19 13:15:01 deraugla Exp $ *)
+(* $Id: Puiseux_base.v,v 1.28 2013-06-19 16:29:38 deraugla Exp $ *)
 
 (* Most of notations are Robert Walker's ones *)
 
@@ -22,8 +22,7 @@ Record field α :=
   { zero : α;
     one : α;
     add : α → α → α;
-    mul : α → α → α
-}.
+    mul : α → α → α }.
 
 (* polynomial of degree ≥ 0 *)
 Record polynomial α := mkpol { al : list α; an : α }.
@@ -51,10 +50,51 @@ Definition den_divides_comden comden p :=
 Definition pow_den_div_com_den α comden (t : term α) :=
   den_divides_comden comden (power t).
 
+Record math_puiseux_series α :=
+  { ms_terms : series α;
+    ms_valuation : Q;
+    ms_comden : positive }.
+
 Record puiseux_series α :=
   { ps_terms : series (term α);
     ps_comden : positive;
     ps_prop : series_forall (pow_den_div_com_den ps_comden) ps_terms }.
+
+Fixpoint terms_of_math_terms α (ms : math_puiseux_series α) z s :=
+  match s with
+  | Term a t =>
+      Term {| coeff := a; power := z # ms_comden ms |}
+        (λ tt, terms_of_math_terms ms (Z.succ z) (t tt))
+  | End =>
+      End (term α)
+  end.
+
+Lemma ps_prop_of_math_loop : ∀ α (ms : math_puiseux_series α) z s t,
+  t = terms_of_math_terms ms z s
+  → series_forall (pow_den_div_com_den (ms_comden ms)) t.
+Proof.
+intros α ms z s t Ht.
+subst t; revert z.
+induction s as [t₁ s₁ IHs| ]; intros.
+ eapply TermAndFurther; [ reflexivity | idtac | apply IHs ].
+ exists z; rewrite Zmult_comm; reflexivity.
+
+ constructor; reflexivity.
+Qed.
+
+Theorem ps_prop_of_math : ∀ α (ms : math_puiseux_series α),
+  series_forall (pow_den_div_com_den (ms_comden ms))
+    (terms_of_math_terms ms 0%Z (ms_terms ms)).
+Proof.
+intros α ms.
+eapply ps_prop_of_math_loop; reflexivity.
+Qed.
+
+Definition puiseux_series_of_math_puiseux_series α
+    (ms : math_puiseux_series α) :=
+  {| ps_terms := terms_of_math_terms ms 0%Z (ms_terms ms);
+     ps_comden := ms_comden ms;
+     ps_prop := ps_prop_of_math ms |}.
 
 Definition valuation α (ps : puiseux_series α) :=
   match series_head (ps_terms ps) with
